\section{L* and NL* execution with example}

This section aims to provide an example of the execution of the two algorithms taking the unknown language $\U$ defined by $\E+(b+aa+abb)(a+b)^*$ % $+(b+aa+abb)(a+b)*
\input{sections/annexe/example/L_example.tex}
\input{sections/annexe/example/NL_example.tex}

\subsection{Example to find residual from a regular language}
In this section I would like to explain why the \textit{mDFA} of \cref{sec:l-exec} has one state more of the \textit{cRFSA} of \cref{sec:nl-exec}.

Let's start with the regular expression of $\U = \E+(b+aa+abb)(a+b)^*$. The residuals of this language can be found iteratively thanks \cref{algo:find_residuals}.


\begin{algorithm}[H]
  \caption{Algo to find residuals of a language $\U$}
  \label{algo:find_residuals}
  \KwIn{$\U$, $\Sigma$}
  \KwOut{$\RE$ = The set of residuals of $\U$}
  $\RE \gets \{\}$ \tcp*{Initialisation of $\RE$}
  $E \gets \{\E\}$\tcp*{The list of words to treat}
  \While{$E.length > 0$}{
    $current \gets E.pop()$\;
    $residual = (current)^{-1}L\footnote{This operation can be performed, for example, with the \textit{Brzozowski derivative} algorithm}$\;
    \If{$residual \notin \RE$}{
      $\RE \gets \RE \cup \{residual\}$\;
      \For{$sym \in \Sigma$}{
        $word \gets current \cdot sym$\;
        $E \gets E \cup \{word\}$\;
      }
    }
  }
  \Return $\RE$
\end{algorithm}

Let's apply this algorithm over $\U$.

\newcommand{\EM}{\varnothing}

\begin{tabular}{c|c|r|l|c|l}
  $Iteration$   & current & Operation      & Result                  & $\RE$                  & $E$                        \\
  \hline\hline
  \textit{Init} & $-$     & $-$            & $-$                     & $\RE = \{\}$           & $E = \{\E\}$               \\
  1             & $\E$    & $\E^{-1}\U$    & $\RE_1 = \U$            & $\RE = \RE \cup \RE_1$ & $E = \{a, b\}$             \\
  2             & $a$     & $a^{-1}\U$     & $\RE_2 = (a+bb)(a+b)^*$ & $\RE = \RE \cup \RE_2$ & $E = \{b, aa, ab\}$        \\
  3             & $b$     & $b^{-1}\U$     & $\RE_3 = (a+b)^*$       & $\RE = \RE \cup \RE_3$ & $E = \{aa, ab, ba, bb\}$   \\
  4             & $aa$    & $(aa)^{-1}\U$  & $(a+b)^* = \RE_3$       & $-$                    & $E = \{ab, ba, bb\}$       \\
  5             & $ab$    & $(ab)^{-1}\U$  & $\RE_4 = b(a+b)^*$      & $\RE = \RE \cup \RE_4$ & $E = \{ba, bb, aba, abb\}$ \\
  6             & $ba$    & $(ba)^{-1}\U$  & $(a+b)^* = \RE_3$       & $-$                    & $E = \{bb, aba, abb\}$     \\
  7             & $bb$    & $(bb)^{-1}\U$  & $(a+b)^* = \RE_3$       & $-$                    & $E = \{aba, abb\}$         \\
  8             & $aba$   & $(aba)^{-1}\U$ & $(a+b)^* = \RE_3$       & $-$                    & $E = \{abb\}$              \\
  9             & $abb$   & $(abb)^{-1}\U$ & $\RE_5 = \EM$           & $\RE = \RE \cup \RE_5$ & $E = \EM$                  \\
\end{tabular}

We see that the residuals of $\U$ are exactly five, the same number of state of the \textit{mDFA} returned by \textit{L*}, but only four of them are \textit{prime} because $\RE_3 = \RE_1 \cup \RE_2 \cup \RE_4$. That's why the \textit{cRFSA} has only four states.